src/QUIC.Impl.Header.fsti
@@ -1,4 +1,6 @@
 module QUIC.Impl.Header
+
+(*
 include QUIC.Spec.Header
 include QUIC.Impl.Base
 
